---
title: "Surds"
language: "en"
previous: "mathContent.html"
---

## Completing the square 

<div markdown="1">
It means that you write the quadratic expression, <p style="display:inline-block">\( ax^2 + bx +c \)</p> in the form a <p style="display:inline-block">\(a(x+p)^2 + q\)</p> where a, b, c, p, and q are real numbers.
<br>
For example, in the expansion of <p style="display:inline-block">\( (x + b)^2 = x^2 + 2bx + b^2 \)</p><br>
Notice that the last term, <p style="display:inline-block">\( b^2 \)</p> is the square of half the coefficient of x, (2b).<br>
</div>

### Method
<div markdown="1">
<br>
	See that the coefficient of <p style="display:inline-block">\( x^2 \)</p> is 1 always, if it is not 1 then adjust the coefficient to 1.<br>
	Add a box squared to bx and subtract a box squared from c. <br>
	Divide the coefficient of x by 2 always, the answer will go in the square boxes.<br>
	Rewrite the expression as <p style="display:inline-block;padding-right:5px;">\( (x + p)^2 + q\)</p>or<p style="display:inline-block;padding-left:5px">\( a(x + p)^2 + q\)</p>
<br>
</div>

### Example:
<div markdown="1">
Complete the square on <p style="display:inline-block">\( x^2 + 6x + 15 \)</p><br>
Answer <br>
<details closed>
  <summary><a>Show Answer</a></summary>
    <p style="display:inline-block">\( x^2 + 6x + 15 = x^2 + 6x + \boxed{}^2 + 15 - \boxed{}^2\)</p><br>
    <p style="display:inline-block">\( = (x + 3)^2 + 15 - 9 \)</p><br>
    <p style="display:inline-block">\( = (x + 3)^2 + 6\)</p><br>
</details>
</div>

### Example:
<div markdown="1">
Complete the square on <p style="display:inline-block">\( 3x^2 + 12x + 27 \)</p><br>
Answer <br>
<details closed>
  <summary><a>Show Answer</a></summary>
    <p style="display:inline-block">\( 3x^2 + 12x + 27 = 3(x^2 + 4x + 9)\)</p><br>
    <p style="display:inline-block">\( = 3((x + 2)^2 + 9 - 2^2) \)</p><br>
    <p style="display:inline-block">\( = 3((x + 2)^2 + 5) \)</p><br>
    <p style="display:inline-block">\( = 3(x + 2)^2 + 15\)</p><br>
</details>
</div>