---
title: "Discriminant"
language: "en"
previous: "solving.html"
---

## Discriminant Function

<div markdown="1">
The discriminant of a quadratic equation is: <p style="display:inline-block">\( \varDelta = b^2 - 4ac \)</p>. <br>
The root of any quadratic equation depends on the discriminant value: <br>
- For one real root the discriminant is 0 (<p style="display:inline-block">\( \varDelta = 0 \)</p>)<br>
- For two real roots the discriminant is greater than 0 (i.e. <p style="display:inline-block">\( \varDelta \gt 0 \)</p>).<br>
- For no roots the discriminant is less than 0 (i.e. <p style="display:inline-block">\( \varDelta \lt 0 \)</p>).

</div> 

## Example of Discriminant Function use

<div markdown="1">
For what values(s) of p does: <p style="display:inline-block padding-right:5px;">\( x^2 + {x \over p} + 1 = 0\) have equal roots</p>.
<details closed>
  <summary><a>Show Answer</a></summary>
    Equal roots means one real root so: <p style="display:inline-block">\(b^2 - 4ac = 0\)</p> <br>
    <p style="display:inline-block">\( ({1 \over p})^2 -4(1)(1) = 0 \)</p>, substitute a = 1, b = 1/p and c = 1 into discriminant equation<br>
    <p style="display:inline-block">\( ({1 \over p})^2 -4 = 0 \)</p><br>
    <p style="display:inline-block">\( ({1 \over p})^2 = 4 \)</p><br>
    <p style="display:inline-block">\( {1 \over p} = 2 \)</p><br>
    <p style="display:inline-block">\( p = {1 \over 2} = 0.5\)</p><br>
</details>
</div> 
<br>
<div markdown="1">
	Find one value of s for which: <p style="display:inline-block padding-right:5px;">\( x^2 + 2(s + 3) x + (s^2 + 2s - 5) \gt 0\), has real roots</p>.
<details closed>
  <summary><a>Show Answer</a></summary>
    Real roots means discrimanant is greater than 0: <p style="display:inline-block">\(b^2 - 4ac = 0\)</p> <br>
    <p style="display:inline-block">\( a = 1\)</p><br>
    <p style="display:inline-block">\( b = 2(s + 3) \)</p><br>
    <p style="display:inline-block">\( c = (s^2 + 2s - 5) \)</p><br>
    <p style="display:inline-block">\( 2(s + 3)^2 - 4(1)(s^2 + 2s - 5) > 0 \)</p>, substitute a = 1, b = 1/p and c = 1 into discriminant equation<br>
    <p style="display:inline-block">\( (2s + 6)(2s + 6) - 4s^2 - 8s + 20 > 0\)</p><br>
    <p style="display:inline-block">\( 4s^2 + 24s + 36 - 4s^2 - 8s + 20 > 0\)</p>, Expand<br>
    <p style="display:inline-block">\( 16s + 56 > 0 \)</p><br>
    <p style="display:inline-block">\( 16s > -56 \)</p><br>
    <p style="display:inline-block">\( s > {-56 \over 16} \)</p><br>
    <p style="display:inline-block">\( s > {-7 \over 2} \)</p><br>
    <p style="display:inline-block">\( s > -3.5 \)</p><br>
</details>
</div> 
