---
title: "Re-arranging Formula"
language: "en"
previous: "complex.html"
---

## Re-arranging Formula

Rearranging formula or rule means we write a given letter in terms of another letter with numbers (.i.e. solve the equation for the unknown).

<div markdown="1">
    <p style="display:inline"> For example, Write \( {(x - 1) \over (x + 1)} = t \) in terms of t </p>.
    <details closed>
      <summary><a>Show Answer</a></summary>
        <p style="display:inline-block">\( {(x - 1) \over (x + 1)} = t \)</p><br>
        Multiply both sides by th denominator (x + 1):<br>
        <p style="display:inline-block">\( x - 1 = t(x + 1) \)</p><br>
        Expand:<br>
        <p style="display:inline-block">\( x - 1 = tx + t \)</p><br>
        Add 1 to each side<br>
        <p style="display:inline-block">\( x = tx + t + 1 \)</p><br>
        Subtract tx from each side<br>
        <p style="display:inline-block">\( x - tx = t + 1 \)</p><br>
        Factorise LHS<br>
        <p style="display:inline-block">\( x(1 - t) = t + 1 \)</p><br>
        Divide both sides by (1 - t)<br>  
        <p style="display:inline-block">\( x = {(t + 1) \over (1 - t)}; t \ne 1\)</p>   
    </details>
</div>
<br>
<div markdown="1">
    <p style="display:inline"> For the given rule \( {y \over (x - 1)} =  {2y \over (3x - 4t)} \) write t as the subject </p>.
    <details closed>
      <summary><a>Show Answer</a></summary>
        <p style="display:inline-block">\( {y \over (x - 1)} =  {2y \over (3x - 4t)}\)</p><br>
        Use fraction multiplying rule: if<p style="display:inline-block">\( {a \over b} = {c \over d}, a * d = c * b\)</p><br>
        <p style="display:inline-block">\( y(3x - 4t) = 2y(x - 1) \)</p><br>
        Divide both sides by y: <br>
        <p style="display:inline-block">\( 3x - 4t = 2(x - 1) \)</p><br>
        Expand: <br>
        <p style="display:inline-block">\( 3x - 4t = 2x - 2 \)</p><br>
        Subtract 3x from both sides: <br>
        <p style="display:inline-block">\( -4t = -x - 2 \)</p><br>
        Divide by -4 <br>
        <p style="display:inline-block">\( t = {-x - 2 \over -4} \)</p><br>
        <p style="display:inline-block">\( t = {x + 2 \over 4} \)</p>
    </details>
</div>


