---
title: "Roots and Coefficients - Relationship Formula"
language: "en"
previous: "index.html"
---

## Relationships between Roots and Coefficients

<div markdown="1">
<p style="display:inline-block">If \( \alpha \) and, \( \beta \)</p> are the roots of the quadratic equation:
<p style="display:inline-block">\( ax^2 + bx + c = 0 \)</p><br>
Then:<br>
<p style="display:inline-block">\( \alpha + \beta = (-b)/a \)</p><br>
<p style="display:inline-block">\( \alpha\beta = c/a \)</p><br>
Proof:<br>
<p style="display:inline-block">\( (x - \alpha)(x - \beta)= x^2 + {b \over a}x + {c \over a} \)</p><br>
<p style="display:inline-block">\( x^2 - (\alpha + \beta)x + \alpha\beta = x^2 + {b \over a}x + {c \over a} \), Simplified</p><br>
Equate the co-efficients on both sides:<br>
<p style="display:inline-block">\( -(\alpha + \beta) = {b \over a} \), Co-efficients of x</p><br>
<p style="display:inline-block">\( \alpha\beta = {c \over a} \), Constant Numbers</p><br>
<br>
<p style="display:inline-block">Suppose that \( \alpha, \beta, and \gamma \), are the roots of a cubic equation of the type \( ax^3 + bx^2 + cx + d = 0\). </p><br> 
By factor theorem, since <p style="display:inline-block"> \( x = \alpha\) is a root of the cubic equation \( (x - \alpha)\) must be a factor and, in a similar way, so must \( (x - \beta) \) and \( (x - \gamma) \).</p><br>
Therefore: <p style="display:inline-block"> \( (x - \alpha)(x - \beta)(x - \gamma) = 0 \) </p><br>
<p style="display:inline-block">By Expanding the brackets and comparing the result with \( ax^3 + bx^2 + cx + d = 0 \), the following results are obtained: </p><br>
<p style="display:inline-block">\( \alpha + \beta + \gamma = {(-b) \over a}\) </p><br>
<p style="display:inline-block">\( \alpha\beta\gamma = {(-d) \over a}\) <br>  

</div>

