---
title: "Surds"
language: "en"
previous: "mathContent.html"
---

## Surds (Roots) 

<div markdown="1" style="display:inline-block">Surds are such expressions as <p style="display:inline-block">\(\sqrt{7}\sqrt[3]{40}\)</p></div> which cannot be evaluated exactly. 
They are irrational. 
Expressions involving surds are simplified. 

### Rules
The following rules apply: 
<div markdown="1">
<p>1. \(\sqrt{a}\ * \sqrt{b}\ = \sqrt{ab}\)</p>
<p>2. \(\sqrt{a}\ \div \sqrt{b}\ = \sqrt{a \div b}\) </p>
<p>3. \(a\sqrt{c} \pm b\sqrt{c} = (a \pm b)\sqrt{c} \) (like surds can be added or subtracted)</p>
Note:
	<p> \(\sqrt{a} * \sqrt{a} = a\)</p>
    <p> \((\sqrt{a})^2 = a\)</p>
	<p> \(\sqrt{a} \pm \sqrt{b}  \ne \sqrt{(a \pm b)}\) for non-zero a and b</p>
</div>

##### To simplify a surd like square roots we have to write the number inside the surd as product of two factors, one factor has to be a largest square number of that surd.
<br>
<div markdown="1">
For Example: <p style="display:inline-block"> \( \sqrt{75} = \sqrt{25 * 3} = \sqrt{25} * \sqrt{3} = 5\sqrt{3} \)</p> <br>
For Example: <p style="display:inline-block"> \( 3\sqrt{2} - \sqrt{8} = 3\sqrt{2} - \sqrt{4 * 2} = 3\sqrt{2} - \sqrt{4} * \sqrt{2} = 3\sqrt{2} - 2\sqrt{2} = \sqrt{2} \)</p> 
</div>


When fractions are involved with surds, it is the normal practice to eliminate the surds from the denominator; this called rationalising the denominator (ie. clearing it of irrational numbers.)
<div markdown="1">
For expression of the type <p style="display:inline-block">\( c \over \sqrt{a} \)</p>, we multiply the top and the bottom by <p style="display:inline-block">\( \sqrt{a} \)</p> giving:
<p style="display:inline-block">\( {c \over \sqrt{a}} = {c \over \sqrt{a}} * {\sqrt{a} \over \sqrt{a}} = {c\sqrt{a} \over a} \)</p>
</div>

## Conjugate Surds
Conjugate surds are surds which will differ in sign,
The rule only applies to binomial (two terms) expressions <br>
A conjugate surd is aquired by replacing the sign with the inverse
For Example:
<div markdown="1">
Binomial Expression <p style="display:inline-block">\( \leftrightarrow \)</p> Corresponding Conjugate 
</div>
<p style="display:inline-block">\( a + \sqrt{b} \leftrightarrow a - \sqrt{b} \)</p><br>
<p style="display:inline-block">\( a - \sqrt{b} \leftrightarrow a + \sqrt{b} \)</p><br>
<p style="display:inline-block">\( \sqrt{a} + b \leftrightarrow \sqrt{a} - b\)</p><br>
<p style="display:inline-block">\( \sqrt{a} - b \leftrightarrow \sqrt{a} + b\)</p><br>

### Simplifying binomial surds written as fraction
<div markdown="1">
Consider <p style="display:inline-block"> \({1 \over b + \sqrt{a}}\)</p>, we multiply the top and the bottom by <p style="display:inline-block"> \(b - \sqrt{a}\)</p>, which is called the conjugate.
<br>
<p style="display:inline-block"> \({1 \over b + \sqrt{a}} = {1 \over (b + \sqrt{a})}  * {b - \sqrt{a} \over b - \sqrt{a}} = {b - \sqrt{a} \over b^2 - (\sqrt{a})^2} = {b - \sqrt{a} \over b^2 - a^2}\)</p>
</div>